LeanApi/Props.lean
@@ -5,3 +5,6 @@ import LeanApi.Props.Sys
 import LeanApi.Props.Ops
 import LeanApi.Props.Store
 import LeanApi.Props.Bridge
+import LeanApi.Props.Registry
+import LeanApi.Props.Authoring
+import LeanApi.Props.Stored
